Common.v and its users: changed lookup to alookup and added aextend.  Changed LEval.v and its dependents to use lists from Common.v.

Common.v
@@ -11,25 +11,44 @@ Module P3Common.
 
 Definition alist (T : Type) : Type := list (id * T).
 
-Fixpoint lookup {X: Type} (x: id) (a: alist X) : option X :=
+Definition aextend {T: Type} (x: id) (v : T) (a: alist T) := (x, v) :: a.
+
+Fixpoint alookup {T: Type} (x: id) (a: alist T) : option T :=
   match a with
     | nil => None
-    | cons (y, v) a' => if eq_id_dec x y then (Some v) else (lookup x a')
+    | cons (y, v) a' => if eq_id_dec y x then (Some v) else (alookup x a')
     end.
 
-Lemma lookup_cons_eq : 
+Lemma alookup_cons_eq : 
   forall T x (v : T) (a : alist T),
-    lookup x (cons (x, v) a) = Some v.
+    alookup x (cons (x, v) a) = Some v.
 Proof.
   intros. simpl. apply eq_id.
 Qed.
 
-Lemma lookup_cons_neq :
+Lemma alookup_cons_neq :
   forall T x y (v : T) (a : alist T),
-    x <> y ->
-    lookup x (cons (y, v) a) = lookup x a.
+    y <> x ->
+    alookup x (cons (y, v) a) = alookup x a.
 Proof.
   intros. simpl. apply neq_id. apply H.
 Qed.
+
+Lemma alookup_aextend_eq : 
+  forall T x (v : T) (a : alist T),
+    alookup x (aextend x v a) = Some v.
+Proof.
+  intros. simpl. apply eq_id.
+Qed.
+
+Lemma alookup_aextend_neq :
+  forall T x y (v : T) (a : alist T),
+    y <> x ->
+    alookup x (aextend y v a) = alookup x a.
+Proof.
+  intros. simpl. apply neq_id. apply H.
+Qed.
+
+Hint Unfold aextend.
 
 End P3Common.
